abstract: simple kernel object getter/setter
- this commit introduces the name "simple kernel object (simple_ko)" for generic (non-arch) kernel objects that are not tcbs or cnodes. For the master l4v, endpoints and notifications are the simple kernel objects.
- simple kernel objects are simple, for instance in the sense that they don't have recursive structure and their validity is defined without using a pointer.
- he setter and getter for simple kernel objects are defined. These replace the specific getters/setters for endpoint and notification. Consequently, almost all wp rules for the two sets of getter/setter are also replaced by the ones for simple kernel object getter/setter.

spec/abstract/Structures_A.thy
@@ -31,6 +31,7 @@ requalify_types
   arch_kernel_obj
   arch_state
   arch_tcb
+  aa_type
 
 requalify_consts
   acap_rights
@@ -49,6 +50,7 @@ requalify_consts
   tcb_bits
   endpoint_bits
   ntfn_bits
+  aa_type
 end
 
 text {*
@@ -456,6 +458,28 @@ where
 | "obj_size (Zombie r zb n) = (case zb of None \<Rightarrow> 1 << obj_bits (TCB undefined)
                                         | Some n \<Rightarrow> 1 << (cte_level_bits + n))"
 | "obj_size (ArchObjectCap a) = 1 << arch_obj_size a"
+
+
+text {* An alternative formulation that allows abstraction over type: *}
+
+datatype a_type =
+    ATCB
+  | AEndpoint
+  | ANTFN
+  | ACapTable nat
+  | AGarbage nat -- "number of bytes of garbage"
+  | AArch aa_type
+
+definition
+  a_type :: "kernel_object \<Rightarrow> a_type"
+where
+ "a_type ob \<equiv> case ob of
+           CNode sz cspace           \<Rightarrow> if well_formed_cnode_n sz cspace
+                                        then ACapTable sz else AGarbage (cte_level_bits + sz)
+         | TCB tcb                   \<Rightarrow> ATCB
+         | Endpoint endpoint         \<Rightarrow> AEndpoint
+         | Notification notification \<Rightarrow> ANTFN
+         | ArchObj ao                \<Rightarrow> AArch (aa_type ao)"
 
 
 section {* Kernel State *}
